`[ltac2 .. ]` notation for `CallLtac2`; `make_ltac2_ref` tactic; static checks

rocq-ltac2-tc-dispatch/tests/arguments.v
@@ -7,8 +7,11 @@ Set Default Proof Mode "Classic".
 
 
 Module LengthMismatch.
-  Definition tac_with_args : nat -> Ltac2Ref.t. constructor. Qed.
+  Definition tac_with_args : nat -> Ltac2Ref.t. make_ltac2_ref. Qed.
   Ltac2 tac_with_args : constr -> constr -> unit -> unit := fun _ _ _ => ().
+  Fail Instance missing_args i b : Dispatch (Nat.eqb i 0 = b) [ltac2 tac_with_args i] := {}.
+
+  (* Ignore static check in [[ltac2]] *)
   Instance missing_args i b : Dispatch (Nat.eqb i 0 = b) (CallLtac2 (tac_with_args i)) := {}.
 
   Goal Nat.eqb 0 0 = true.
@@ -16,11 +19,11 @@ Module LengthMismatch.
     Fail goal_dispatch.
   Abort.
 
-  Definition tac_with_args_fixed : nat -> bool -> Ltac2Ref.t. constructor. Qed.
+  Definition tac_with_args_fixed : nat -> bool -> Ltac2Ref.t. make_ltac2_ref. Qed.
   Ltac2 tac_with_args_fixed : constr -> constr -> unit -> unit :=
     fun i b () =>
       refine '(@eq_refl _ _ :> (Nat.eqb $i 0 = $b)).
-  Instance dispatch_with_args i b : Dispatch (Nat.eqb i 0 = b) (CallLtac2 (tac_with_args_fixed i b)) | 100 := {}.
+  Instance dispatch_with_args i b : Dispatch (Nat.eqb i 0 = b) [ltac2 tac_with_args_fixed i b] | 100 := {}.
 
   Goal Nat.eqb 0 0 = true.
   Proof.
@@ -33,8 +36,11 @@ Module LengthMismatch.
 End LengthMismatch.
 
 Module TypeMismatch.
-  Definition tac_with_args : nat -> Ltac2Ref.t. constructor. Qed.
+  Definition tac_with_args : nat -> Ltac2Ref.t. make_ltac2_ref. Qed.
   Ltac2 tac_with_args : unit -> unit -> unit := fun _ _ => ().
+  Fail Instance missing_args i b : Dispatch (Nat.eqb i 0 = b) [ltac2 tac_with_args i] := {}.
+
+  (* Ignore static check in [[ltac2]] *)
   Instance missing_args i b : Dispatch (Nat.eqb i 0 = b) (CallLtac2 (tac_with_args i)) := {}.
 
   Goal Nat.eqb 0 0 = true.
@@ -43,11 +49,11 @@ Module TypeMismatch.
   Abort.
 End TypeMismatch.
 
-Definition tac_with_args : nat -> bool -> Ltac2Ref.t. constructor. Qed.
+Definition tac_with_args : nat -> bool -> Ltac2Ref.t. make_ltac2_ref. Qed.
 Ltac2 tac_with_args : constr -> constr -> unit -> unit :=
   fun i b () =>
     refine '(@eq_refl _ _ :> (Nat.eqb $i 0 = $b)).
-Instance dispatch_with_args i b : Dispatch (Nat.eqb i 0 = b) (CallLtac2 (tac_with_args i b)) := {}.
+Instance dispatch_with_args i b : Dispatch (Nat.eqb i 0 = b) [ltac2 tac_with_args i b] := {}.
 
 Goal Nat.eqb 0 0 = true.
 Proof.
@@ -60,12 +66,12 @@ Proof.
   goal_dispatch.
 Qed.
 
-Definition test_reduction : nat -> nat -> Ltac2Ref.t. constructor. Qed.
+Definition test_reduction : nat -> nat -> Ltac2Ref.t. make_ltac2_ref. Qed.
 Ltac2 test_reduction : constr -> constr -> unit -> unit :=
   fun i j () =>
     Control.assert_true (Bool.neg (Constr.equal i j));
     refine 'eq_refl.
-Instance test_reduction_inst i j : Dispatch (i = j) (CallLtac2 (test_reduction i j)) := {}.
+Instance test_reduction_inst i j : Dispatch (i = j) [ltac2 test_reduction i j] := {}.
 
 Goal 1 + 2 = 3 + 0.
 Proof.
