rocq-ltac2-tc-dispatch/tests/nested.v
@@ -1,11 +1,11 @@
 Require Import skylabs.ltac2.tc_dispatch.lookup.
 
 Module Import Nested.
-  Definition inside_module : Ltac2Ref.t. constructor. Qed.
+  Definition inside_module : Ltac2Ref.t. make_ltac2_ref. Qed.
   Import Printf.
   Ltac2 inside_module () :=
     ltac1:(reflexivity).
-  Instance nested_inst : Dispatch (0 = 0) (CallLtac2 inside_module) := {}.
+  Instance nested_inst : Dispatch (0 = 0) [ltac2 inside_module] := {}.
 End Nested.
 
 Example test_success_nested : 0 = 0.
