rocq-ltac2-tc-dispatch/tests/simple.v
@@ -1,11 +1,11 @@
 Require Import skylabs.ltac2.tc_dispatch.lookup.
 
 (* A simple success tactic *)
-Definition solve_true : Ltac2Ref.t. constructor. Qed.
+Definition solve_true : Ltac2Ref.t. make_ltac2_ref. Qed.
 Ltac2 solve_true () := ltac1:(exact I).
 
 (* Success Instance for True *)
-Instance test_true_inst : Dispatch True (CallLtac2 solve_true) := {}.
+Instance test_true_inst : Dispatch True [ltac2 solve_true] := {}.
 
 Example test_succeed : True.
 Proof.
@@ -21,24 +21,25 @@ Abort.
 Inductive Broken : nat -> Prop :=.
 
 Section BrokenSection.
-  Variable X : Ltac2Ref.t.
+  Variable X : Prop.
+  (* [make_ltac2_ref] checks that the reference does not depend on section variables. *)
+  Definition tac (x : X) : Ltac2Ref.t. Fail make_ltac2_ref. Abort.
+  Definition tac (T : Type) : Ltac2Ref.t. make_ltac2_ref. Qed.
 
-  (* A "Broken" Instance: will be generalized *)
-  #[global] Instance broken_inst : Dispatch (Broken 0) (CallLtac2 X) := {}.
+  (* Ltac2 [tac] does not exist yet. *)
+  Fail #[global] Instance broken_inst : Dispatch (Broken 0) [ltac2 tac] := {}.
+
+  Ltac2 tac := fun () => ().
+
+  (* Type mismatch: tac expects no arguments *)
+  Fail #[global] Instance broken_inst : Dispatch (Broken 0) [ltac2 (tac nat)] := {}.
+
+  (* We can circumvent the check in the [[ltac2]] notation by using [CallLtac2] directly *)
+  #[global] Instance broken_inst : Dispatch (Broken 0) (CallLtac2 (tac nat)) := {}.
+  (* But the resulting hint will not work because our definition [tac] takes
+     more arguments than the [tac] tactic. *)
+  Example test_fail_bad_string : Broken 0.
+  Proof.
+    Fail goal_dispatch.
+  Abort.
 End BrokenSection.
-
-(* Generalized [Lta2Ref] *)
-Example test_fail_bad_string : Broken 0.
-Proof.
-  Fail goal_dispatch. (* Triggers the None branch of our match *)
-Abort.
-
-(* Applied [Ltac2Ref]s are not supported *)
-Definition broken_ref : nat -> Ltac2Ref.t. constructor. Qed.
-Instance broken_inst_applied : Dispatch (Broken 1) (CallLtac2 (broken_ref 1)) := {}.
-
-(* Applied [Ltac2Ref] *)
-Example test_fail_bad_string : Broken 1.
-Proof.
-  Fail goal_dispatch. (* Triggers the None branch of our match *)
-Abort.
