rocq-ltac2-tc-dispatch/tests/external.v
@@ -1,7 +1,7 @@
 Require Import Ltac2.Ltac2.
 Require Import skylabs.ltac2.tc_dispatch.lookup.
 
-Definition ext_tactic : Ltac2Ref.t. constructor. Qed.
+Definition ext_tactic : Ltac2Ref.t. ltac1:(make_ltac2_ref). Qed.
 Ltac2 ext_tactic () := ltac1:(reflexivity).
 
 #[export]
