rocq-ltac2-tc-dispatch/theories/lookup.v
@@ -13,14 +13,23 @@ Require Import skylabs.ltac2.logger.logger.
 
 Declare ML Module "ltac2-tc-dispatch.plugin".
 
-Module Ltac2Ref.
-  (** [Ltac2Ref.t] is a trivial inductive type used to store names of Ltac2
-      tactics via proxy constants. Recommended use:
-      <<
-        Definition my_tactic : Ltac2Ref.t. constructor. Qed.
-      >>
-   *)
-  Inductive t := _mk.
+#[global] Reserved Notation "'[ltac2' t ]" (format "[ltac2  t ]").
+
+Module Type LTAC2_REF.
+  Parameter t : Prop.
+  Parameter _mk : t.
+End LTAC2_REF.
+
+(** [Ltac2Ref.t] is a trivial inductive type used to store names of Ltac2
+    tactics via proxy constants. The constructor [_mk] is not meant to be used
+    directly. Instead, use the [make_ltac2_ref] tactic which ensures that the
+    reference being built does not depend on section variables.
+    << Definition my_tactic : Ltac2Ref.t. make_ltac2_ref. Qed. >>
+ *)
+Module Ltac2Ref : LTAC2_REF.
+  Inductive _t := __mk.
+  Definition t := _t.
+  Definition _mk := __mk.
 End Ltac2Ref.
 
 (** [Handler goal] represents strategies to apply to goals matching the type
@@ -48,6 +57,15 @@ Module ltac2.
   Ltac2 @ external resolve_ltac2 : reference -> constr list -> (unit -> unit) option :=
     "ltac2_tc_dispatch" "resolve_ltac2".
 
+  Ltac2 check_constant (c : constr) :=
+    match Constr.Unsafe.kind c with
+    | Constr.Unsafe.Constant r _ => ConstRef r
+    | _ =>
+        let msg := fprintf "[ltac2_tac] must refer to a constant. Found: %t" c in
+        log[tc_dispatch, 1] "%m" msg;
+        Control.zero (Tactic_failure (Some msg))
+  end.
+
   Ltac2 goal_dispatch_with (dbs : ident list option) :=
     let g := Control.goal () in
     let query := open_constr:(Dispatch $g _) in
@@ -70,13 +88,7 @@ Module ltac2.
     in
     let (r, args) :=
       let (h, args) := Constr.decompose_app c in
-      match Constr.Unsafe.kind h with
-      | Constr.Unsafe.Constant r _ => (ConstRef r, Array.to_list args)
-      | _ =>
-          let msg := fprintf "[ltac2_tac] must refer to a constant without arguments. Found: %t" c in
-          log[tc_dispatch, 1] "%m" msg;
-          Control.zero (Tactic_failure (Some msg))
-      end
+      (check_constant h, Array.to_list args)
     in
     match resolve_ltac2 r args with
     | Some f => f ()
@@ -84,10 +96,53 @@ Module ltac2.
         let msg := fprintf "Could not find Ltac2 tactic: %t" c in
         log[tc_dispatch, 1] "%m" msg;
         Control.zero (Tactic_failure (Some msg))
-    end
-  .
+    end.
 
-  #[global] Ltac2 Notation "goal_dispatch" dbs(opt(seq("with", list0(ident)))) := goal_dispatch_with dbs.
+  Ltac2 check_ref () :=
+  (* We want to make sure that no section variables are used. There might be
+     arguments already introduced. We revert all non-section variables and check
+     that the resulting type does not depend on section variables. *)
+    let hyps := Control.hyps () in
+    let to_revert :=
+      let f (i, _, _) := if Control.is_section_variable i then None else Some i in
+      List.map_filter f hyps
+    in
+    Std.revert to_revert;
+    let g := Control.goal () in
+    let deps := Constr.Vars.vars_really_needed g in
+    let f v :=
+      if Control.is_section_variable v then
+        let msg := fprintf "Signature %t depends on section variable %I" g v in
+        Control.zero (Invalid_argument (Some msg))
+      else
+        ()
+    in
+    List.iter f (FSet.elements deps).
+
+  Ltac2 check_ref_use (t : preterm) :=
+    let t := Constr.pretype t in
+    let (h, args) := Constr.decompose_app t in
+    let r := check_constant h in
+    match resolve_ltac2 r (Array.to_list args) with
+    | Some _ =>
+        let vars := Constr.Vars.vars_really_needed t in
+        let f v :=
+          if Control.is_section_variable v then
+            let msg := fprintf "Ltac2Ref %t depends on section variable %I" h v in
+            Control.zero (Invalid_argument (Some msg))
+          else
+            ()
+        in
+        List.iter f (FSet.elements vars);
+        Control.refine (fun _ => t)
+    | None =>
+        let msg := fprintf "Could not find Ltac2 tactic: %t" h in
+        log[tc_dispatch, 1] "%m" msg;
+        Control.zero (Invalid_argument (Some msg))
+    end.
+
+  #[global] Ltac2 Notation "goal_dispatch" dbs(opt(seq("with", list0(ident)))) :=
+    goal_dispatch_with dbs.
 
   Ltac2 goal_dispatch_with_ltac1 (dbs : Ltac1.t option) :=
     let dbs :=
@@ -106,6 +161,12 @@ Module ltac2.
   Ltac goal_dispatch :=
     ltac2:(goal_dispatch_with None).
 End ltac2.
+
+Ltac make_ltac2_ref :=
+  ltac2:(ltac2.check_ref ()); intros; exact Ltac2Ref._mk.
+
+#[global] Notation "'[ltac2' t ]" := (CallLtac2 ltac2:(ltac2.check_ref_use t)) (only parsing).
+#[global] Notation "'[ltac2' t ]" := (CallLtac2 t) (only printing).
 
 Tactic Notation "goal_dispatch" "with" ident_list(dbs) :=
   ltac2.goal_dispatch_with dbs.
